src/Misc.v
@@ -5,6 +5,11 @@ Proof.
   unfold Proper, respectful; intros; apply Nat.add_le_mono; assumption.
 Qed.
 
+#[global] Instance Proper_mul_le : Proper (le ==> le ==> le) Nat.mul.
+Proof.
+  unfold Proper, respectful; intros; apply Nat.mul_le_mono; assumption.
+Qed.
+
 #[global] Instance Proper_sub_le : Proper (le ==> eq ==> le) Nat.sub.
 Proof.
   unfold Proper, respectful; intros; subst; apply Nat.sub_le_mono_r; assumption.
